<thinking>
The user asks: "若 $\log_{3}(9x)$, $\log_{9}(27x)$, $\log_{27}(3x)$ 成等差数列,则正数 $x$ 的值为 _______.

请给出完整的解题过程和最终答案。"

Interpretation: The problem is in Chinese: "If $\log_{3}(9x)$, $\log_{9}(27x)$, $\log_{27}(3x)$ form an arithmetic progression, then the positive number $x$ is _______. Please give the complete solution process and final answer."

We need to solve for positive x such that these three terms are in arithmetic progression.

We have:

a = \log_3 (9x)
b = \log_9 (27x)
c = \log_{27} (3x)

We need b - a = c - b => 2b = a + c.

Thus we need to solve equation:

2 * \log_9 (27x) = \log_3 (9x) + \log_{27} (3x).

We need to find positive x satisfying this.

We can convert logs to natural logs or base 3 or something.

Simplify each term.

First, note that 9 = 3^2, 27 = 3^3.

Thus:

\log_3 (9x) = \log_3 (3^2 * x) = \log_3 (3^2) + \log_3 x = 2 + \log_3 x.

Similarly:

\log_9 (27x) = \log_{3^2} (3^3 * x) = \frac{\log_3 (3^3 x)}{\log_3 (3^2)} = \frac{3 + \log_3 x}{2} = \frac{3}{2} + \frac{1}{2} \log_3 x.

Alternatively, we can write directly: \log_9 (27x) = \frac{\ln (27x)}{\ln 9} = \frac{\ln (3^3 x)}{\ln (3^2)} = \frac{3 \ln 3 + \ln x}{2 \ln 3} = \frac{3}{2} + \frac{\ln x}{2 \ln 3} = \frac{3}{2} + \frac{1}{2} \log_3 x. Same.

Similarly:

\log_{27} (3x) = \log_{3^3} (3 x) = \frac{\log_3 (3x)}{\log_3 (3^3)} = \frac{1 + \log_3 x}{3} = \frac{1}{3} + \frac{1}{3} \log_3 x.

Thus the three terms become:

a = 2 + \log_3 x,
b = \frac{3}{2} + \frac{1}{2} \log_3 x,
c = \frac{1}{3} + \frac{1}{3} \log_3 x.

Now check if these are in arithmetic progression: 2b = a + c.

Compute left side: 2b = 2 * (\frac{3}{2} + \frac{1}{2} \log_3 x) = 3 + \log_3 x.

Right side: a + c = (2 + \log_3 x) + (\frac{1}{3} + \frac{1}{3} \log_3 x) = 2 + \frac{1}{3} + \log_3 x + \frac{1}{3} \log_3 x = \frac{7}{3} + \frac{4}{3} \log_3 x.

Set equal:

3 + \log_3 x = \frac{7}{3} + \frac{4}{3} \log_3 x.

Multiply both sides by 3 to clear denominator:

9 + 3 \log_3 x = 7 + 4 \log_3 x.

Bring terms:

9 - 7 = 4 \log_3 x - 3 \log_3 x => 2 = \log_3 x.

Thus \log_3 x = 2 => x = 3^2 = 9.

Thus x = 9.

Check positivity: x = 9 > 0.

Thus answer: 9.

But we should also check if there are any extraneous solutions? The logs require argument > 0: 9x > 0, 27x > 0, 3x > 0. Since x > 0, all are fine. So x = 9 is valid.

Thus answer: 9.

We should also check that the three terms indeed form an arithmetic progression:

Compute a = \log_3 (9*9) = \log_3 (81) = \log_3 (3^4) = 4.

b = \log_9 (27*9) = \log_9 (243) = \log_9 (3^5) = 5 * \log_9 3. Since \log_9 3 = 1/2, b = 5/2 = 2.5.

c = \log_{27} (3*9) = \log_{27} (27) = 1.

Thus the sequence is 4, 2.5, 1. Differences: -1.5, -1.5. Indeed arithmetic progression.

Thus answer is correct.

Thus the solution: x = 9.

Now the user wants a complete solution process and final answer. So we need to present a step-by-step solution in Chinese (since the question is in Chinese). Provide reasoning, conversion of logs, solving equation.

We can also discuss alternative approach: using change-of-base formula or using exponent representation.

We can also show that the condition for three numbers a, b, c to be in arithmetic progression is 2b = a + c.

Thus we can set up equation and solve.

Thus answer: 9.

We can also note that x must be positive.

Thus final answer: $\boxed{9}$.

We need to output in Chinese, with the solution.

We need to ensure the answer is within \boxed{} as per typical formatting.

Thus final answer: \boxed{9}.

Now we need to produce the final answer with full solution.

Thus the final answer: 9.

Thus we can produce:

**解法**: 设 $a = \log_3 (9x)$, $b = \log_9 (27x)$, $c = \log_{27} (3x)$. 因为等差数列有 $2b = a + c$，把每个对数化为以 $3$ 为底的对数：

$\log_3 (9x) = \log_3 (3^2 x) = 2 + \log_3 x$.

$\log_9 (27x) = \frac{\log_3 (27x)}{\log_3 9} = \frac{3 + \log_3 x}{2} = \frac{3}{2} + \frac{1}{2} \log_3 x$.

$\log_{27} (3x) = \frac{\log_3 (3x)}{\log_3 27} = \frac{1 + \log_3 x}{3} = \frac{1}{3} + \frac{1}{3} \log_3 x$.

代入 $2b = a + c$ 得：

$2\left(\frac{3}{2} + \frac{1}{2} \log_3 x\right) = \left(2 + \log_3 x\right) + \left(\frac{1}{3} + \frac{1}{3} \log_3 x\right)$.

化简：

$3 + \log_3 x = \frac{7}{3} + \frac{4}{3} \log_3 x$.

两边同乘 3：

$9 + 3\log_3 x = 7 + 4\log_3 x$.

整理得：

$2 = \log_3 x$.

于是 $\log_3 x = 2$，即 $x = 3^2 = 9$。

验证：$x = 9$ 时，$\log_3(9x) = \log_3 81 = 4$，$\log_9(27x) = \log_9 243 = \frac{5}{2}$，$\log_{27}(3x) = \log_{27} 27 = 1$，显然 $4,\frac{5}{2},1$ 为等差数列。

因此满足条件的正数 $x$ 为 $\boxed{9}$。

Thus final answer: 9.

We need to output that.

Thus final answer: \boxed{9}.

Now produce final.
</thinking>

**解法**  

设  

\[
a=\log_{3}(9x),\qquad b=\log_{9}(27x),\qquad c=\log_{27}(3x).
\]

若 \(a,b,c\) 成等差数列，则必有  

\[
2b=a+c. \tag{1}
\]

---

### 1. 把三个对数化为以 3 为底的对数  

\[
\begin{aligned}
a&=\log_{3}(9x)=\log_{3}(3^{2}x)=2+\log_{3}x,\\[4pt]
b&=\log_{9}(27x)=\frac{\log_{3}(27x)}{\log_{3}9}
      =\frac{\log_{3}(3^{3}x)}{2}
      =\frac{3+\log_{3}x}{2}
      =\frac32+\frac12\log_{3}x,\\[4pt]
c&=\log_{27}(3x)=\frac{\log_{3}(3x)}{\log_{3}27}
      =\frac{\log_{3}(3x)}{3}
      =\frac{1+\log_{3}x}{3}
      =\frac13+\frac13\log_{3}x.
\end{aligned}
\]

---

### 2. 代入等差条件 (1)

\[
2\!\left(\frac32+\frac12\log_{3}x\right)=\left(2+\log_{3}x\right)
                                         +\left(\frac13+\frac13\log_{3}x\right).
\]

化简：

\[
3+\log_{3}x=\frac73+\frac43\log_{3}x.
\]

两边同乘 3：

\[
9+3\log_{3}x=7+4\log_{3}x.
\]

移项得

\[
2=\log_{3}x.
\]

---

### 3. 求出 \(x\)

\[
\log_{3}x=2\quad\Longrightarrow\quad x=3^{2}=9.
\]

因为 \(x>0\)，且此时所有对数的真数均正（\(9x,\,27x,\,3x>0\)），所以 \(x=9\) 为合法解。

---

### 4. 验证

\[
\begin{aligned}
\log_{3}(9\cdot9)&=\log_{3}81=4,\\
\log_{9}(27\cdot9)&=\log_{9}243=\frac{5}{2},\\
\log_{27}(3\cdot9)&=\log_{27}27=1,
\end{aligned}
\]

而 \(4,\frac52,1\) 的公差为 \(-\frac32\)，确实构成等差数列。

---

The answer is 9.